aaa

fold.v
@@ -43,39 +43,194 @@ Proof.
   rewrite !H0; auto.
 Qed.
 
-Variable len : nat.
-Hypothesis len_is_power_of_2 : exists e : nat, len = 2 ^ len.
-
 Notation " p '>>1'" := (Ediv2 p) (at level 40, left associativity) : exp_scope.
 
 Definition If (b : bexp) (c : cmd) := Cif b c.
 
 Variable ntrd : nat.
 Hypothesis ntrd_neq_0 : ntrd <> 0.
+Hypothesis ntrd_is_p2 : exists e : nat, ntrd = 2 ^ e.
 
-Definition arr_val_compat (s : nat) (len : nat) (f fc : nat -> Z) :=
-  match s with
-    | O => fc 0 = sum_of len f
-    | _ => sum_of (len / 2) fc = sum_of len f
+Definition arr_val_compat (len : nat) (f : nat -> Z) (sum : Z) :=
+  match len with
+    | O => f 0 = sum
+    | _ => sum_of len f = sum
   end.
 
-Definition INV (i : nat) :=
-  Ex (s e st : nat) (fc : nat -> Z),
+Variable f : nat -> Z.
+
+Definition INV :=
+  Ex (i s e : nat) (fc : nat -> Z),
+    !(TID === Enum' i) **
     !(St === Enum' s) **
     !(pure (s = Div2.div2 (2 ^ e))) **
+    !(pure (arr_val_compat (2 * s) fc (sum_of (2 * ntrd) f))) **
+    !(pure (s <= ntrd)) **
     (if Nat.eq_dec s 0 then
-       !(pure (len = s * st)) ** nth i (distribute 1 (ARR + TID) len fc (nt_step 1) 0) emp
+       nth i (distribute 1 ARR (2 * ntrd) fc (nt_step 1) 0) emp
      else
-       nth i (distribute s (ARR + TID) len fc (nt_step s) 0) emp).
+       nth i (distribute s ARR (2 * ntrd) fc (nt_step s) 0) emp).
 
 Definition fold_ker :=
-  S ::= Enum' len >>1 ;;
-  WhileI FalseP ( Enum' 0 < S ) (
-    If ( Evar TID < S ) (
+  St ::= Enum' ntrd ;;
+  WhileI (INV) ( Enum' 0 < St ) (
+    If ( Evar TID < St ) (
       T1 ::= [ ARR + TID ] ;;
-      T2 ::= [ ARR + TID + S ] ;;
+      T2 ::= [ ARR + TID + St ] ;;
       [ ARR + TID ] ::= T1 + T2
     ) (SKIP) ;;
-    S ::= S >>1 ;;
+    St ::= St >>1 ;;
     Cbarrier 0
-  )%exp.           
+  )%exp.
+
+Definition binv0 : Vector.t assn ntrd * Vector.t assn ntrd :=
+  (MyVector.init (fun i : Fin.t ntrd =>
+   let tid := nat_of_fin i in
+   Ex s fc, 
+     !(St === Enum' s) **
+     !(pure (arr_val_compat (2 * ntrd) fc (sum_of (2 * ntrd) f))) **
+       let tid := nat_of_fin i in
+       nth tid (distribute (2 * s) ARR (2 * ntrd) fc (nt_step (2 * s)) 0) emp),
+   MyVector.init (fun i => 
+   let tid := nat_of_fin i in
+   Ex s fc, 
+     !(St === Enum' s) **
+     !(pure (arr_val_compat (2 * ntrd) fc (sum_of (2 * ntrd) f))) **
+       let tid := nat_of_fin i in
+       nth tid (distribute s ARR (2 * ntrd) fc (nt_step s) 0) emp)).
+
+Lemma arr_compat_same (len : nat) (fc : nat -> Z) :
+  len <> 0 -> arr_val_compat len fc (sum_of len fc).
+Proof.
+  induction len; simpl in *; auto; omega.
+Qed.
+Require Import SetoidClass.
+Instance app_proper (s : stack) (h : pheap) : Proper (equiv_sep ==> iff) (fun P => P s h).
+Proof.
+  intros P Q H.
+  specialize (H s h); auto.
+Qed.
+
+Ltac fold_pure H s :=
+  lazymatch type of H with
+    | ?X =>
+      let Hf := fresh in
+      assert (Hf : !(pure X) s emp_ph) by (apply pure_emp; [auto|apply emp_emp_ph]);
+        clear H; rename Hf into H
+end.
+
+Ltac rewrite_sep_in lem H :=
+  match type of H with
+    | ?X _ _ => pattern X in H
+  end; rewrite lem in H; cbv beta in H. 
+
+Theorem fold_ker_correct (tid : Fin.t ntrd) : 
+  CSL (fun i => match i with O => binv0 | _ => default ntrd end) tid
+  (nth (nat_of_fin tid) (distribute ntrd ARR (2 * ntrd) f (nt_step ntrd) 0) emp **
+   !(TID === Z_of_fin tid))
+  fold_ker
+  (Ex fc,
+     nth (nat_of_fin tid) (distribute ntrd ARR (2 * ntrd) f (nt_step 1) 0) emp **
+     !(pure (fc 0 = sum_of (2 * ntrd) f))).
+Proof.
+  unfold fold_ker.
+  assert (Htid : nat_of_fin tid < ntrd) by (destruct (Fin.to_nat tid); simpl in *; try omega).
+  remember (2 * ntrd) eqn:Hntrd2.
+
+  eapply rule_seq.
+  { hoare_forward.
+    simpl; intros ? ? [v H].
+    eapply scRw in H; [|intros ? ? H'; subA_normalize_in H'; exact H' | intros ? ? H'; exact H'].
+    simpl in H; exact H. }
+
+  hoare_forward.
+  Focus 3.
+  { unfold INV. intros s h H.
+    destruct ntrd_is_p2 as [e Hntrd].
+    exists (nat_of_fin tid), (ntrd), (S e), f.
+    sep_split_in H; sep_split; auto.
+    - rewrite Nat.pow_succ_r', Div2.div2_double; unfold_conn; auto.
+    - apply arr_compat_same; omega.
+    - red; auto.
+    - destruct (Nat.eq_dec _ _); [omega | congruence]. } Unfocus.
+
+  eapply Hbackward.
+  Focus 2.
+  { unfold INV; intros s h H.
+    sep_split_in H; destruct H as (i & st & e & fc & H).
+    sep_combine_in H.
+    ex_intro i H; ex_intro st H; ex_intro e H; ex_intro fc H; simpl in H.    
+    exact H. } Unfocus.
+  
+  apply rule_ex; intros fc.
+  apply rule_ex; intros e.
+  apply rule_ex; intros st.
+  apply rule_ex; intros i.
+  
+  eapply rule_seq.
+
+  eapply rule_if_disj.
+  { eapply Hbackward.
+    Focus 2.
+    { unfold INV; intros s h H.
+      sep_split_in H.
+
+      Ltac change_in H :=
+        lazymatch type of H with
+          | _ ?s ?h =>
+            let P := fresh "P" in 
+            let Hf := fresh "H" in
+            evar (P : assn); assert (Hf : P s h); unfold P in *; clear P; [| clear H; rename Hf into H]
+        end.
+      change_in H.
+      { red in HP0, HP1, HP2; simpl in HP0, HP1, HP2.
+        destruct Z_lt_dec; [|congruence]. destruct Nat.eq_dec; [omega|].
+        subst; remember (2 * ntrd) as n eqn:Hntrd2.
+        cutrewrite (0 = 0 * st) in H; [|auto].
+        red in HP, HP5; simpl in HP, HP5; destruct (Z_lt_dec); try congruence.
+        apply skip_arr_unfold' in H; try omega; simpl in H.
+        cutrewrite (st + 0 = 1 * st) in H; [|omega].
+        rewrite_sep_in skip_arr_unfold' H; try omega.
+        rewrite mult_1_l in H; exact H. }
+      sep_combine_in H.
+      exact H. } Unfocus.
+    
+    eapply rule_seq.
+    { repeat hoare_forward. 
+      apply inde_distribute; repeat (constructor; auto).
+      intros ? ? H; exact H. }
+    
+    eapply rule_seq.
+    { cutrewrite (Z.of_nat (st + i) = Z.of_nat st + Z.of_nat i)%Z; [|apply Nat2Z.inj_add].
+      hoare_forward. 
+      apply inde_distribute; repeat (constructor; auto).
+      intros ? ? H; exact H. }
+    
+    { hoare_forward.
+      intros ? ? H; exact H. } }
+  
+  apply rule_skip.
+
+  eapply Hforward.
+  eapply rule_disj.
+  - eapply rule_seq; [hoare_forward|].
+    { intros s h H.
+      destruct H as [st' H].
+      subA_normalize_in H. simpl in H.
+      ex_intro st' H; exact H. }
+
+    hoare_forward. 
+    lazymatch goal with
+    | [ |- CSL ?bspec ?tid ?P (Cbarrier ?i) ?Q] =>
+    eapply Hbackward; [
+        eapply Hforward; [
+          eapply rule_frame; 
+          [eapply rule_barrier | prove_inde] |
+           autounfold; simpl; repeat rewrite MyVector.init_spec in *] | 
+        (*frame_analysis (Vector.nth (fst (bspec i)) tid)*)] end.
+  Focus 2.
+  simpl; rewrite MyVector.init_spec.
+  intros s h H.
+  sep_normal_in H; sep_split_in H.
+   
+    
